theories/Compositional_Structures/Basic_Modules/Component_Types/Electoral_Module_Ref.thy
@@ -8,6 +8,16 @@ begin
 
 type_synonym 'a Electoral_Module_Ref = "'a set \<Rightarrow> 'a Profile_List \<Rightarrow> 'a Result nres"
 
+abbreviation elec_mod_rel_orig :: "('a \<times> 'a) set \<Rightarrow> 
+  (('a set \<Rightarrow> 'a Profile \<Rightarrow> 'a Result) \<times> ('a set \<Rightarrow> 'a Profile \<Rightarrow> 'a Result)) set" where
+  "elec_mod_rel_orig R \<equiv> \<langle>\<langle>R\<rangle>set_rel , \<langle>\<langle>\<langle>R \<times>\<^sub>r R\<rangle>set_rel\<rangle>list_rel , 
+  \<langle>R\<rangle>set_rel \<times>\<^sub>r \<langle>R\<rangle>set_rel \<times>\<^sub>r \<langle>R\<rangle>set_rel\<rangle>fun_rel\<rangle>fun_rel" 
+
+abbreviation elec_mod_rel_ref :: "('a \<times> 'a) set \<Rightarrow> 
+  (('a set \<Rightarrow> 'a Profile_List \<Rightarrow> 'a Result) \<times> ('a set \<Rightarrow> 'a Profile_List \<Rightarrow> 'a Result)) set" where
+  "elec_mod_rel_ref R \<equiv> \<langle>\<langle>R\<rangle>set_rel , \<langle>\<langle>\<langle>R\<rangle>list_rel\<rangle>list_rel , 
+  \<langle>R\<rangle>set_rel \<times>\<^sub>r \<langle>R\<rangle>set_rel \<times>\<^sub>r \<langle>R\<rangle>set_rel\<rangle>fun_rel\<rangle>fun_rel" 
+
 abbreviation elec_mod_relb :: "('a \<times> 'a) set \<Rightarrow> ('a Electoral_Module_Ref \<times> ('a set \<Rightarrow> 'a Profile \<Rightarrow> 'a Result nres)) set" where
   "elec_mod_relb R \<equiv> \<langle>R\<rangle>alt_set_rel \<rightarrow> profile_rel 
   \<rightarrow> \<langle>\<langle>R\<rangle>set_rel \<times>\<^sub>r \<langle>R\<rangle>set_rel \<times>\<^sub>r \<langle>R\<rangle>set_rel\<rangle>nres_rel"
