theories/Compositional_Structures/Sepref_Bindings.thy
@@ -1,0 +1,38 @@
+theory Sepref_Bindings
+  imports "Basic_Modules/Borda_Module_Ref"
+    "Basic_Modules/Condorcet_Module_Ref"
+    Sequential_Composition_Ref
+
+begin
+
+
+
+sepref_decl_op (no_def) borda_mod: "borda_ref :: 'a Electoral_Module_Ref" :: "elec_mod_rel_ref Id"
+  apply standard
+  apply (rule nres_relI)
+  apply simp
+  done
+
+sepref_decl_op (no_def) borda_doit: "borda :: 'a Electoral_Module" :: "elec_mod_rel_orig Id"
+  apply standard
+  apply (rule nres_relI)
+  apply simp
+  done
+  
+
+  context 
+    notes alts_assn_def[symmetric,fcomp_norm_unfold] 
+       profile_assn_def[symmetric,fcomp_norm_unfold]
+       result_set_assn_def[symmetric,fcomp_norm_unfold]
+ alts_ref_assn_def[symmetric,fcomp_norm_unfold] ballot_ref_assn_def[symmetric,fcomp_norm_unfold]
+      
+begin
+
+
+sepref_decl_impl borda_impl: borda_elim_sepref.refine[FCOMP borda_ref_correct] 
+  unfolding alts_ref_assn_def .
+
+
+
+                                                
+end
